Normalization_Definitions.thy
@@ -7,42 +7,76 @@ The only reason these are here instead of in their respective
   normalization files is to reduce dependencies across files.
   This benefits development on my low-RAM laptop.\<close>
 
-(* TODO figure out a way to remove this reduncancy with the locales *)
-lemma "wf_ast_problem p \<longleftrightarrow> ast_problem.wf_problem p"
-  by (simp add: wf_ast_problem_def)
-
 text \<open> Input Restriction \<close>
 
 (* TODO think of a better name *)
-abbreviation "\<omega> \<equiv> Either [''object'']"
+abbreviation "\<omega> \<equiv> Either [STR ''object'']"
 
 (* This being omitted from wf_action_schema complicates type normalization *)
-definition (in ast_domain) wf_action_params :: "ast_action_schema \<Rightarrow> bool" where
-  "wf_action_params a \<equiv> (\<forall>(n, t) \<in> set (parameters a). wf_type t)"
-
+definition (in domain_signature) wf_action_params :: "ast_classical_action_schema \<Rightarrow> bool" where
+  "wf_action_params a \<equiv> (\<forall>(n, t) \<in> set (parameters (head a)). wf_type t)"
+ 
 fun single_type :: "type \<Rightarrow> bool" where
   "single_type (Either ts) \<longleftrightarrow> length ts = 1"
 abbreviation single_types :: "('a \<times> type) list \<Rightarrow> bool" where
   "single_types os \<equiv> \<forall>(_, T) \<in> set os. single_type T"
 
-definition (in ast_domain) restrict_dom :: bool where
-  "restrict_dom \<equiv> single_types (consts D)
-                  \<and> list_all1 wf_action_params (actions D)"
+definition (in domain_signature) restrict_dom_sig where
+  "restrict_dom_sig \<equiv> single_types consts"
 
-locale restrict_domain = wf_ast_domain +
+definition (in ast_classical_domain) restrict_dom where
+  "restrict_dom \<equiv> restrict_dom_sig \<and> (\<forall>a \<in> set (actions D). wf_action_params a)"
+
+definition (in problem_signature) restrict_prob_sig where
+  "restrict_prob_sig \<equiv> restrict_dom_sig \<and> single_types objs"
+
+definition (in ast_classical_problem) restrict_prob where
+  "restrict_prob \<equiv> restrict_dom \<and> single_types (objects P)"
+
+locale restrict_domain_signature = domain_signature +
+  assumes restrict_dom_sig: restrict_dom_sig
+
+locale restrict_problem_signature = problem_signature +
+  assumes restrict_prob_sig: restrict_prob_sig
+
+locale restrict_classical_domain = wf_ast_classical_domain +
   assumes restrict_dom: restrict_dom
-lemmas restrict_domain_def' =
-  restrict_domain_def[unfolded wf_ast_domain_def restrict_domain_axioms_def]
 
-definition (in ast_problem) "restrict_prob \<equiv> restrict_dom \<and> single_types (objects P)"
-
-locale restrict_problem = wf_ast_problem +
+locale restrict_classical_problem = wf_ast_classical_problem +
   assumes restrict_prob: restrict_prob
-lemmas restrict_problem_def' =
-  restrict_problem_def[unfolded wf_ast_problem_def restrict_problem_axioms_def]
 
-sublocale restrict_problem \<subseteq> restrict_domain "D"
-  using restrict_prob restrict_prob_def by (unfold_locales) simp
+sublocale restrict_problem_signature \<subseteq> restrict_domain_signature
+  using restrict_prob_sig restrict_prob_sig_def
+  by unfold_locales blast
+
+sublocale restrict_classical_domain \<subseteq> restrict_domain_signature 
+    "types D" "predicates D" "functions D" "consts D"
+  using restrict_dom restrict_dom_def restrict_dom_sig_def
+  by unfold_locales blast
+
+sublocale restrict_classical_problem \<subseteq> restrict_classical_domain D
+  using restrict_prob restrict_prob_def
+  by unfold_locales blast
+ 
+sublocale restrict_classical_problem \<subseteq> restrict_problem_signature
+    "types D" "predicates D" "functions D" "consts D" "objects P"
+  using restrict_prob restrict_prob_def restrict_dom_def restrict_prob_sig_def
+  by unfold_locales blast
+
+text \<open>Combined well-formed + restricted signatures. These are convenient to use as a single
+  context for proofs that need both the \<open>wf_\<close> assumption and the \<open>restrict_\<close> assumption.\<close>
+
+locale wf_restrict_domain_signature = wf_domain_signature + restrict_domain_signature
+
+locale wf_restrict_problem_signature = wf_problem_signature + restrict_problem_signature
+
+sublocale wf_restrict_problem_signature \<subseteq> wf_restrict_domain_signature ..
+
+sublocale restrict_classical_domain \<subseteq>
+  wf_restrict_domain_signature "types D" "predicates D" "functions D" "consts D" ..
+
+sublocale restrict_classical_problem \<subseteq>
+  wf_restrict_problem_signature "types D" "predicates D" "functions D" "consts D" "objects P" ..
 
 
 text \<open> Type normalization:
@@ -54,78 +88,111 @@ text \<open> Type normalization:
   - const types are Either [''object'']
   - actions parameters are detyped
     This isn't superfluous because wf_action_schema does not ensure well-formed param types. \<close>
-definition (in ast_domain) "typeless_dom \<equiv>
-    types D = []
-    \<and> (\<forall>p \<in> set (predicates D). \<forall>T \<in> set (argTs p). T = \<omega>)
-    \<and> (\<forall>(n, T) \<in> set (consts D). T = \<omega>)
+
+definition (in domain_signature) "typeless_domain_signature \<equiv>
+  ty_decl = []
+  \<and> (\<forall>p \<in> set predicates. \<forall>T \<in> set (predicate_decl.argTs p). T = \<omega>)
+  \<and> (\<forall>f \<in> set functions. \<forall>T \<in> set (function_decl.argTs f). T = \<omega>)
+  \<and> (\<forall>(n, T) \<in> set consts. T = \<omega>)"
+
+locale typeless_domain_signature = domain_signature + 
+  assumes typeless_domain_signature: typeless_domain_signature
+
+definition (in problem_signature) "typeless_problem_signature \<equiv>
+  typeless_domain_signature
+  \<and> (\<forall>(n, T) \<in> set objs. T = \<omega>)"
+
+locale typeless_problem_signature = problem_signature +
+  assumes typeless_problem_signature: typeless_problem_signature
+
+sublocale typeless_problem_signature \<subseteq> typeless_domain_signature
+  using typeless_problem_signature typeless_problem_signature_def
+  by unfold_locales simp
+
+definition (in ast_classical_domain) "typeless_classical_domain \<equiv>
+    typeless_domain_signature
     \<and> (\<forall>ac \<in> set (actions D). \<forall>(n, T) \<in> set (ac_params ac). T = \<omega>)"
 
-(*locale typeless_domain = wf_ast_domain +
-  assumes typeless_dom: typeless_dom
-lemmas typeless_domain_def' =
-  typeless_domain_def[unfolded wf_ast_domain_def typeless_domain_axioms_def]*)
+locale typeless_classical_domain = wf_ast_classical_domain +
+  assumes typeless_classical_domain: typeless_classical_domain
+
+sublocale typeless_classical_domain \<subseteq> typeless_domain_signature "types D" "predicates D" "functions D" "consts D"
+  using typeless_classical_domain typeless_classical_domain_def
+  by unfold_locales simp
+
+lemmas typeless_classical_domain_def' =
+  typeless_classical_domain_def[unfolded wf_ast_classical_domain_def typeless_classical_domain_axioms_def]
 
 text \<open>
 - domain is detyped
 - objects are detyped \<close>
-definition (in ast_problem) "typeless_prob \<equiv>
-  typeless_dom \<and> (\<forall>(n, T) \<in> set (objects P). T = \<omega>)"
 
-(*locale typeless_problem = wf_ast_problem +
-  assumes typeless_prob: typeless_prob
-lemmas typeless_problem_def' =
-  typeless_problem_def[unfolded wf_ast_problem_def typeless_problem_axioms_def]
+definition (in ast_classical_problem) "typeless_classical_problem \<equiv>
+  typeless_classical_domain \<and> (\<forall>(n, T) \<in> set (objects P). T = \<omega>)"
 
-sublocale typeless_problem \<subseteq> typeless_domain D
-  using typeless_prob typeless_prob_def by (unfold_locales) blast *)
+locale typeless_classical_problem = wf_ast_classical_problem +
+  assumes typeless_classical_problem: typeless_classical_problem
+lemmas typeless_classical_problem_def' =
+  typeless_classical_problem_def[unfolded wf_ast_classical_problem_def typeless_classical_problem_axioms_def]
+
+sublocale typeless_classical_problem \<subseteq> typeless_classical_domain D
+  using typeless_classical_problem typeless_classical_problem_def by (unfold_locales) blast
+
+sublocale typeless_classical_problem \<subseteq> 
+    typeless_problem_signature "types D" "predicates D" "functions D" "consts D" "objects P"
+  apply unfold_locales
+  using typeless_classical_problem 
+  unfolding typeless_classical_problem_def typeless_classical_domain_def 
+  unfolding typeless_domain_signature_def typeless_problem_signature_def
+  by simp
 
 text \<open> Precondition normalization: all action preconditions are normalized. \<close>
 
-definition (in ast_domain) "prec_normed_dom \<equiv> \<forall>ac \<in> set (actions D). is_conj (ac_pre ac)"
+definition (in ast_classical_domain) "prec_normed_dom \<equiv> \<forall>ac \<in> set (actions D). is_conj (ac_pre ac)"
 
-(*locale precond_normed_domain = wf_ast_domain +
+(*locale precond_normed_domain = wf_ast_classical_domain +
   assumes prec_normed_dom: prec_normed_dom
 lemmas precond_normed_domain_def' =
-  precond_normed_domain_def[unfolded wf_ast_domain_def precond_normed_domain_axioms_def]*)
+  precond_normed_domain_def[unfolded wf_ast_classical_domain_def precond_normed_domain_axioms_def]*)
 
 text \<open> Preconditions only exist in the domain, so no additional definition is needed for the problem.\<close>
 
-(*locale precond_normed_problem = wf_ast_problem +
+(*locale precond_normed_problem = wf_ast_classical_problem +
   assumes prec_normed_prob: prec_normed_dom
 lemmas precond_normed_problem_def' =
-  precond_normed_problem_def[unfolded wf_ast_problem_def precond_normed_problem_axioms_def]
+  precond_normed_problem_def[unfolded wf_ast_classical_problem_def precond_normed_problem_axioms_def]
 
 sublocale precond_normed_problem \<subseteq> precond_normed_domain D
   using prec_normed_prob by (unfold_locales) simp*)
 
 text \<open> Complete normalization additionally assumes that the goal is a conjunction. \<close>
 
-definition (in ast_domain) "normalized_dom \<equiv> typeless_dom \<and> prec_normed_dom"
+definition (in ast_classical_domain) "normalized_dom \<equiv> typeless_classical_domain \<and> prec_normed_dom"
 
-locale normalized_domain = wf_ast_domain +
+locale normalized_domain = wf_ast_classical_domain +
   assumes normalized_dom: normalized_dom
 lemmas normalized_domain_def' =
-  normalized_domain_def[unfolded wf_ast_domain_def normalized_domain_axioms_def]
+  normalized_domain_def[unfolded wf_ast_classical_domain_def normalized_domain_axioms_def]
 
-(*sublocale normalized_domain \<subseteq> typeless_domain D
+(*sublocale normalized_domain \<subseteq> typeless_classical_domain D
   using normalized_dom normalized_dom_def by (unfold_locales) simp
 
 sublocale normalized_domain \<subseteq> precond_normed_domain D
   using normalized_dom normalized_dom_def by (unfold_locales) simp*)
 
-definition (in ast_problem) "normalized_prob \<equiv>
-  typeless_prob \<and> prec_normed_dom \<and> is_conj (goal P)"
+definition (in ast_classical_problem) "normalized_prob \<equiv>
+  typeless_classical_problem \<and> prec_normed_dom \<and> is_conj (goal P)"
 
-locale normalized_problem = wf_ast_problem +
+locale normalized_problem = wf_ast_classical_problem +
   assumes normalized_prob: normalized_prob
 lemmas normalized_problem_def' =
-  normalized_problem_def[unfolded wf_ast_problem_def normalized_problem_axioms_def]
+  normalized_problem_def[unfolded wf_ast_classical_problem_def normalized_problem_axioms_def]
 
 sublocale normalized_problem \<subseteq> normalized_domain D
-  using normalized_prob normalized_dom_def normalized_prob_def typeless_prob_def
+  using normalized_prob normalized_dom_def normalized_prob_def typeless_classical_problem_def
   by (unfold_locales) blast
 
-(*sublocale normalized_problem \<subseteq> typeless_problem P
+(*sublocale normalized_problem \<subseteq> typeless_classical_problem P
   using normalized_prob normalized_prob_def by (unfold_locales) simp
 
 sublocale normalized_problem \<subseteq> precond_normed_problem P
@@ -133,13 +200,13 @@ sublocale normalized_problem \<subseteq> precond_normed_problem P
 
 text \<open> Relaxation \<close>
 
-definition (in ast_domain) "relaxed_dom \<equiv>
+definition (in ast_classical_domain) "relaxed_dom \<equiv>
   normalized_dom \<and> (\<forall>a \<in> set (actions D). is_pos_conj (ac_pre a))"
 
 locale relaxed_domain = normalized_domain +
   assumes relaxed_dom: relaxed_dom
 
-definition (in ast_problem) "relaxed_prob \<equiv> normalized_prob \<and>
+definition (in ast_classical_problem) "relaxed_prob \<equiv> normalized_prob \<and>
   is_pos_conj (goal P) \<and> (\<forall>a \<in> set (actions D). is_pos_conj (ac_pre a))"
 
 locale relaxed_problem = normalized_problem +
@@ -148,15 +215,15 @@ locale relaxed_problem = normalized_problem +
 sublocale relaxed_problem \<subseteq> relaxed_domain D
   using relaxed_prob normalized_dom relaxed_prob_def relaxed_dom_def
   by (unfold_locales) simp
-
+(* 
 subsection \<open> Reachability Definitions \<close>
 text \<open> A plan action is applicable if there exists some plan that executes it.
   Whether or not this plan actually solves the task doesn't matter.\<close>
-
-definition (in ast_problem) applicable :: "plan_action \<Rightarrow> bool"
+(
+definition (in ast_classical_problem) applicable :: "plan_action \<Rightarrow> bool"
   where "applicable \<pi> \<equiv> \<exists>\<pi>s M. plan_action_path I \<pi>s M \<and> \<pi> \<in> set \<pi>s"
 
-lemma (in ast_problem) applicable_alt:
+lemma (in ast_classical_problem) applicable_alt:
   "applicable \<pi> \<longleftrightarrow> (\<exists>\<pi>s M. plan_action_path I \<pi>s M \<and>
     plan_action_enabled \<pi> M)"
 proof
@@ -181,23 +248,23 @@ qed
 
 text \<open> A fact is achievable if there exists some plan that results in a state containing it. \<close>
 
-definition (in ast_problem) achievable :: "object atom formula \<Rightarrow> bool"
+definition (in ast_classical_problem) achievable :: "object atom formula \<Rightarrow> bool"
   where "achievable a \<equiv> \<exists>\<pi>s M. plan_action_path I \<pi>s M \<and> a \<in> M"
 
-lemma (in wf_ast_problem) init_achievable:
+lemma (in wf_ast_classical_problem) init_achievable:
   "\<forall>a \<in> set (init P). achievable a"
 proof -
   have "plan_action_path I [] I" by simp
   thus ?thesis unfolding achievable_def I_def by blast
 qed
 
-lemma (in wf_ast_problem) achievable_wf:
+lemma (in wf_ast_classical_problem) achievable_wf:
   "achievable a \<Longrightarrow> wf_fmla_atom objT a"
   unfolding achievable_def
   using wf_I wf_plan_action_path
   unfolding wf_world_model_def by meson
 
-lemma (in wf_ast_problem) achievable_predAtm:
+lemma (in wf_ast_classical_problem) achievable_predAtm:
   "achievable a \<Longrightarrow> is_predAtom a"
   using achievable_wf wf_fmla_atom_alt by blast
 
@@ -214,19 +281,19 @@ fun grounded_pred :: "predicate_decl \<Rightarrow> bool" where
 fun grounded_ac :: "ast_action_schema \<Rightarrow> bool" where
   "grounded_ac (Action_Schema n params pre effs) \<longleftrightarrow> params = []"
 
-definition (in ast_domain) "grounded_dom \<equiv>
+definition (in ast_classical_domain) "grounded_dom \<equiv>
   types D = [] \<and>
   list_all1 grounded_pred (predicates D) \<and>
   consts D = [] \<and>
   list_all1 grounded_ac (actions D)"
 
-locale grounded_domain = wf_ast_domain +
+locale grounded_domain = wf_ast_classical_domain +
   assumes grounded_dom: grounded_dom
 
-definition (in ast_problem) "grounded_prob \<equiv>
+definition (in ast_classical_problem) "grounded_prob \<equiv>
   grounded_dom \<and> objects P = []"
 
-locale grounded_problem = wf_ast_problem +
+locale grounded_problem = wf_ast_classical_problem +
   assumes grounded_prob: grounded_prob
 
 sublocale grounded_problem \<subseteq> grounded_domain D
@@ -263,6 +330,6 @@ locale grounded_normalized_problem = grounded_problem +
 
 sublocale grounded_normalized_problem \<subseteq> grounded_normalized_domain D
   using normed_prob by (unfold_locales) blast
-
+  *)
 
 end
