Running_Example.thy
@@ -1,8 +1,6 @@
 theory Running_Example
   imports Main
     Grounding_Pipeline
-    "AI_Planning_Languages_Semantics.PDDL_STRIPS_Checker"
-    PDDL_Checker_Utils
 begin
 
 subsection \<open> Problem Description \<close>
@@ -23,178 +21,193 @@ It can't use, because I restrict that:
 \<close>
 
 definition "my_types \<equiv> [
-  (''City'', ''object''), (''Movable'', ''object''),
-  (''Vehicle'', ''Movable''), (''Parcel'', ''Movable''),
-  (''Car'', ''Vehicle''), (''Train'', ''Vehicle''),
-  (''R'', ''L''), (''L'', ''R''),
-  (''Batmobile'', ''Car''), (''Batmobile'', ''Train'')]"
+  (STR ''City'', STR ''object''), (STR ''Movable'', STR ''object''),
+  (STR ''Vehicle'', STR ''Movable''), (STR ''Parcel'', STR ''Movable''),
+  (STR ''Car'', STR ''Vehicle''), (STR ''Train'', STR ''Vehicle''),
+  (STR ''R'', STR ''L''), (STR ''L'', STR ''R''),
+  (STR ''Batmobile'', STR ''Car''), (STR ''Batmobile'', STR ''Train'')]"
 (* purposely doing Car/Train instead of only Vehicle, for no reason other than to just use that feature somewhere *)
 definition "my_preds \<equiv> [
-  PredDecl (Pred ''at'') [Either [''Movable''], Either [''City'']],
-  PredDecl (Pred ''in'') [Either [''Parcel''], Either [''Car'', ''Train'']],
-  PredDecl (Pred ''road'') [Either [''City''], Either [''City'']],
-  PredDecl (Pred ''rails'') [Either [''City''], Either [''City'']]
+  PredDecl (Pred STR ''at'') [Either [STR ''Movable''], Either [STR ''City'']],
+  PredDecl (Pred STR ''in'') [Either [STR ''Parcel''], Either [STR ''Car'', STR ''Train'']],
+  PredDecl (Pred STR ''road'') [Either [STR ''City''], Either [STR ''City'']],
+  PredDecl (Pred STR ''rails'') [Either [STR ''City''], Either [STR ''City'']]
 ]"
 definition "my_consts \<equiv> [
-  (Obj ''A'', Either [''City'']), (Obj ''B'', Either [''City'']),
-  (Obj ''C'', Either [''City'']), (Obj ''D'', Either [''City'']),
-  (Obj ''E'', Either [''City'']), (Obj ''F'', Either [''City'']),
-  (Obj ''G'', Either [''City''])
+  (Obj STR ''A'', Either [STR ''City'']), (Obj STR ''B'', Either [STR ''City'']),
+  (Obj STR ''C'', Either [STR ''City'']), (Obj STR ''D'', Either [STR ''City'']),
+  (Obj STR ''E'', Either [STR ''City'']), (Obj STR ''F'', Either [STR ''City'']),
+  (Obj STR ''G'', Either [STR ''City''])
 ]"
 
-definition "op_drive \<equiv> Action_Schema ''drive''
-  [(Var ''c'', Either [''Car'']), (Var ''from'', Either [''City'']), (Var ''to'', Either [''City''])]
-  (And (Atom (predAtm (Pred ''at'') [term.VAR (Var ''c''), term.VAR (Var ''from'')]))
-     (Or (Atom (predAtm (Pred ''road'') [term.VAR (Var ''from''), term.VAR (Var ''to'')]))
-         (Atom (predAtm (Pred ''road'') [term.VAR (Var ''to''), term.VAR (Var ''from'')]))))
-  (Effect
-    [Atom (predAtm (Pred ''at'') [term.VAR (Var ''c''), term.VAR (Var ''to'')])]
-    [Atom (predAtm (Pred ''at'') [term.VAR (Var ''c''), term.VAR (Var ''from'')])])"
-definition "op_choochoo \<equiv> Action_Schema ''choochoo''
-  [(Var ''t'', Either [''Train'']), (Var ''from'', Either [''City'']), (Var ''to'', Either [''City''])]
-  (And (Atom (predAtm (Pred ''at'') [term.VAR (Var ''t''), term.VAR (Var ''from'')]))
-     (Or (Atom (predAtm (Pred ''rails'') [term.VAR (Var ''from''), term.VAR (Var ''to'')]))
-         (Atom (predAtm (Pred ''rails'') [term.VAR (Var ''to''), term.VAR (Var ''from'')]))))
-  (Effect
-    [Atom (predAtm (Pred ''at'') [term.VAR (Var ''t''), term.VAR (Var ''to'')])]
-    [Atom (predAtm (Pred ''at'') [term.VAR (Var ''t''), term.VAR (Var ''from'')])])"
+definition "op_drive \<equiv> SimpleActionSchema
+  (ActionHead STR ''drive''
+    [(Var STR ''c'', Either [STR ''Car'']), (Var STR ''from'', Either [STR ''City'']), (Var STR ''to'', Either [STR ''City''])])
+  (SimpleActionBody
+    (And (Atom (predAtm (Pred STR ''at'') [term.VAR (Var STR ''c''), term.VAR (Var STR ''from'')]))
+       (Or (Atom (predAtm (Pred STR ''road'') [term.VAR (Var STR ''from''), term.VAR (Var STR ''to'')]))
+           (Atom (predAtm (Pred STR ''road'') [term.VAR (Var STR ''to''), term.VAR (Var STR ''from'')]))))
+    (Effect
+      [Atom (predAtm (Pred STR ''at'') [term.VAR (Var STR ''c''), term.VAR (Var STR ''to'')])]
+      [Atom (predAtm (Pred STR ''at'') [term.VAR (Var STR ''c''), term.VAR (Var STR ''from'')])] []))"
+definition "op_choochoo \<equiv> SimpleActionSchema
+  (ActionHead STR ''choochoo''
+    [(Var STR ''t'', Either [STR ''Train'']), (Var STR ''from'', Either [STR ''City'']), (Var STR ''to'', Either [STR ''City''])])
+  (SimpleActionBody
+    (And (Atom (predAtm (Pred STR ''at'') [term.VAR (Var STR ''t''), term.VAR (Var STR ''from'')]))
+       (Or (Atom (predAtm (Pred STR ''rails'') [term.VAR (Var STR ''from''), term.VAR (Var STR ''to'')]))
+           (Atom (predAtm (Pred STR ''rails'') [term.VAR (Var STR ''to''), term.VAR (Var STR ''from'')]))))
+    (Effect
+      [Atom (predAtm (Pred STR ''at'') [term.VAR (Var STR ''t''), term.VAR (Var STR ''to'')])]
+      [Atom (predAtm (Pred STR ''at'') [term.VAR (Var STR ''t''), term.VAR (Var STR ''from'')])] []))"
 (* into has to be Car/Train instead of Vehicle because of the definition of the predicate "in" *)
-definition "op_load \<equiv> Action_Schema ''load''
-  [(Var ''what'', Either [''Parcel'']), (Var ''where'', Either [''City'']), (Var ''into'', Either [''Car'', ''Train''])]
-     (And (Atom (predAtm (Pred ''at'') [term.VAR (Var ''into''), term.VAR (Var ''where'')]))
-         (Atom (predAtm (Pred ''at'') [term.VAR (Var ''what''), term.VAR (Var ''where'')])))
-  (Effect
-    [Atom (predAtm (Pred ''in'') [term.VAR (Var ''what''), term.VAR (Var ''into'')])]
-    [Atom (predAtm (Pred ''at'') [term.VAR (Var ''what''), term.VAR (Var ''where'')])])"
-definition "op_unload \<equiv> Action_Schema ''unload''
-  [(Var ''what'', Either [''Parcel'']), (Var ''from'', Either [''Car'', ''Train'']), (Var ''where'', Either [''City''])]
-     (And (Atom (predAtm (Pred ''at'') [term.VAR (Var ''from''), term.VAR (Var ''where'')]))
-         (Atom (predAtm (Pred ''in'') [term.VAR (Var ''what''), term.VAR (Var ''from'')])))
-  (Effect
-    [Atom (predAtm (Pred ''at'') [term.VAR (Var ''what''), term.VAR (Var ''where'')])]
-    [Atom (predAtm (Pred ''in'') [term.VAR (Var ''what''), term.VAR (Var ''from'')])])"
+definition "op_load \<equiv> SimpleActionSchema
+  (ActionHead STR ''load''
+    [(Var STR ''what'', Either [STR ''Parcel'']), (Var STR ''where'', Either [STR ''City'']), (Var STR ''into'', Either [STR ''Car'', STR ''Train''])])
+  (SimpleActionBody
+     (And (Atom (predAtm (Pred STR ''at'') [term.VAR (Var STR ''into''), term.VAR (Var STR ''where'')]))
+         (Atom (predAtm (Pred STR ''at'') [term.VAR (Var STR ''what''), term.VAR (Var STR ''where'')])))
+    (Effect
+      [Atom (predAtm (Pred STR ''in'') [term.VAR (Var STR ''what''), term.VAR (Var STR ''into'')])]
+      [Atom (predAtm (Pred STR ''at'') [term.VAR (Var STR ''what''), term.VAR (Var STR ''where'')])] []))"
+definition "op_unload \<equiv> SimpleActionSchema
+  (ActionHead STR ''unload''
+    [(Var STR ''what'', Either [STR ''Parcel'']), (Var STR ''from'', Either [STR ''Car'', STR ''Train'']), (Var STR ''where'', Either [STR ''City''])])
+  (SimpleActionBody
+     (And (Atom (predAtm (Pred STR ''at'') [term.VAR (Var STR ''from''), term.VAR (Var STR ''where'')]))
+         (Atom (predAtm (Pred STR ''in'') [term.VAR (Var STR ''what''), term.VAR (Var STR ''from'')])))
+    (Effect
+      [Atom (predAtm (Pred STR ''at'') [term.VAR (Var STR ''what''), term.VAR (Var STR ''where'')])]
+      [Atom (predAtm (Pred STR ''in'') [term.VAR (Var STR ''what''), term.VAR (Var STR ''from'')])] []))"
 (* btw, this is considered well-formed as long as x is not used in precondition or effects *)
-definition "op_broken \<equiv> Action_Schema ''broken''
-  [(Var ''x'', Either [''n'existe pas''])]
-  \<bottom>
-  (Effect [] [])"
+definition "op_broken \<equiv> SimpleActionSchema
+  (ActionHead STR ''broken''
+    [(Var STR ''x'', Either [STR ''n'existe pas''])])
+  (SimpleActionBody \<bottom> (Effect [] [] []))"
 (* This operator is only there to demonstrate relaxation of action preconditions, since I couldn't think of anything
   better that would make use of negative preconditions.*)
-definition "op_build_tracks \<equiv> Action_Schema ''lay_tracks''
-  [(Var ''from'', Either [''City'']), (Var ''to'', Either [''City''])]
-  (And (Not (Atom (predAtm (Pred ''rails'') [term.VAR (Var ''from''), term.VAR (Var ''to'')])))
-       (Not (Atom (predAtm (Pred ''rails'') [term.VAR (Var ''to''), term.VAR (Var ''from'')]))))
-  (Effect [Atom (predAtm (Pred ''rails'') [term.VAR (Var ''from''), term.VAR (Var ''to'')])] [])"
+definition "op_build_tracks \<equiv> SimpleActionSchema
+  (ActionHead STR ''lay_tracks''
+    [(Var STR ''from'', Either [STR ''City'']), (Var STR ''to'', Either [STR ''City''])])
+  (SimpleActionBody
+    (And (Not (Atom (predAtm (Pred STR ''rails'') [term.VAR (Var STR ''from''), term.VAR (Var STR ''to'')])))
+         (Not (Atom (predAtm (Pred STR ''rails'') [term.VAR (Var STR ''to''), term.VAR (Var STR ''from'')]))))
+    (Effect [Atom (predAtm (Pred STR ''rails'') [term.VAR (Var STR ''from''), term.VAR (Var STR ''to'')])] [] []))"
 
+definition "my_funcs \<equiv> []"
 
 definition "my_actions \<equiv> [op_drive, op_choochoo, op_load, op_unload]"
 
-definition "my_domain \<equiv> Domain my_types my_preds my_consts my_actions"
+definition "my_domain \<equiv> Domain my_types my_preds my_funcs my_consts my_actions"
 value "my_domain"
 
 (* batmobile because why not *)
 definition "my_objs \<equiv> [
-  (Obj ''c1'', Either [''Car'']),
-  (Obj ''c2'', Either [''Car'']),
-  (Obj ''c3'', Either [''Car'']),
-  (Obj ''t'', Either [''Train'']),
-  (Obj ''p1'', Either [''Parcel'']),
-  (Obj ''p2'', Either [''Parcel'']),
-  (Obj ''batmobile'', Either [''Batmobile''])
+  (Obj STR ''c1'', Either [STR ''Car'']),
+  (Obj STR ''c2'', Either [STR ''Car'']),
+  (Obj STR ''c3'', Either [STR ''Car'']),
+  (Obj STR ''t'', Either [STR ''Train'']),
+  (Obj STR ''p1'', Either [STR ''Parcel'']),
+  (Obj STR ''p2'', Either [STR ''Parcel'']),
+  (Obj STR ''batmobile'', Either [STR ''Batmobile''])
 ]"
 
-abbreviation fact_to_atm :: "(name \<times> string list) \<Rightarrow> object atom formula" where
+abbreviation fact_to_atm :: "(name \<times> String.literal list) \<Rightarrow> object atom formula" where
   "fact_to_atm f \<equiv> case f of (p, xs) \<Rightarrow> Atom (predAtm (Pred p) (map Obj xs))"
 
 definition "my_init \<equiv> [
-  Atom (predAtm (Pred ''at'') [Obj ''c1'', Obj ''A'']),
-  Atom (predAtm (Pred ''at'') [Obj ''c2'', Obj ''B'']),
-  Atom (predAtm (Pred ''at'') [Obj ''c3'', Obj ''G'']),
-  Atom (predAtm (Pred ''at'') [Obj ''t'', Obj ''E'']),
-  Atom (predAtm (Pred ''at'') [Obj ''p1'', Obj ''C'']),
-  Atom (predAtm (Pred ''at'') [Obj ''p2'', Obj ''F'']),
-  Atom (predAtm (Pred ''road'') [Obj ''A'', Obj ''D'']),
-  Atom (predAtm (Pred ''road'') [Obj ''B'', Obj ''D'']),
-  Atom (predAtm (Pred ''road'') [Obj ''C'', Obj ''D'']),
-  Atom (predAtm (Pred ''rails'') [Obj ''D'', Obj ''E'']),
-  Atom (predAtm (Pred ''road'') [Obj ''E'', Obj ''F'']),
-  Atom (predAtm (Pred ''road'') [Obj ''F'', Obj ''G'']),
-  Atom (predAtm (Pred ''road'') [Obj ''G'', Obj ''E''])
+  Atom (predAtm (Pred STR ''at'') [Obj STR ''c1'', Obj STR ''A'']),
+  Atom (predAtm (Pred STR ''at'') [Obj STR ''c2'', Obj STR ''B'']),
+  Atom (predAtm (Pred STR ''at'') [Obj STR ''c3'', Obj STR ''G'']),
+  Atom (predAtm (Pred STR ''at'') [Obj STR ''t'', Obj STR ''E'']),
+  Atom (predAtm (Pred STR ''at'') [Obj STR ''p1'', Obj STR ''C'']),
+  Atom (predAtm (Pred STR ''at'') [Obj STR ''p2'', Obj STR ''F'']),
+  Atom (predAtm (Pred STR ''road'') [Obj STR ''A'', Obj STR ''D'']),
+  Atom (predAtm (Pred STR ''road'') [Obj STR ''B'', Obj STR ''D'']),
+  Atom (predAtm (Pred STR ''road'') [Obj STR ''C'', Obj STR ''D'']),
+  Atom (predAtm (Pred STR ''rails'') [Obj STR ''D'', Obj STR ''E'']),
+  Atom (predAtm (Pred STR ''road'') [Obj STR ''E'', Obj STR ''F'']),
+  Atom (predAtm (Pred STR ''road'') [Obj STR ''F'', Obj STR ''G'']),
+  Atom (predAtm (Pred STR ''road'') [Obj STR ''G'', Obj STR ''E''])
 ]"
 (* purposefully omitting batmobile from init because that would
   increase the ground problem too much *)
-(* Atom (predAtm (Pred ''at'') [Obj ''batmobile'', Obj ''D'']) *)
+(* Atom (predAtm (Pred STR ''at'') [Obj STR ''batmobile'', Obj STR ''D'']) *)
 
 definition "my_goal \<equiv>
-  And (Atom (predAtm (Pred ''at'') [Obj ''p1'', Obj ''G'']))
-      (Atom (predAtm (Pred ''at'') [Obj ''p2'', Obj ''E'']))"
+  And (Atom (predAtm (Pred STR ''at'') [Obj STR ''p1'', Obj STR ''G'']))
+      (Atom (predAtm (Pred STR ''at'') [Obj STR ''p2'', Obj STR ''E'']))"
 
 definition "my_problem \<equiv> Problem my_domain my_objs my_init my_goal"
 
-lemma wf_d1: "ast_domain.wf_domain my_domain"
-  by (intro wf_domain_intro) eval
+(* lemma wf_d1: "wf_ast_classical_domain my_domain"
+  apply unfold_locales
+  unfolding ast_classical_domain.wf_classical_domain_def 
+  unfolding domain_signature.wf_domain_signature_def
+  unfolding domain_signature.wf_types_def
+  
 
 lemma wf_p1: "ast_problem.wf_problem my_problem"
-  by (intro wf_problem_intro) eval
+  by (intro wf_problem_intro) eval *)
 
 subsection \<open> Execution \<close>
 
 definition "my_plan \<equiv> [
-  PAction ''drive'' [Obj ''c1'', Obj ''A'', Obj ''D''],
-  PAction ''drive'' [Obj ''c1'', Obj ''D'', Obj ''C''],
-  PAction ''load'' [Obj ''p1'', Obj ''C'', Obj ''c1''],
-  PAction ''drive'' [Obj ''c1'', Obj ''C'', Obj ''D''],
-  PAction ''unload'' [Obj ''p1'', Obj ''c1'', Obj ''D''],  
-  PAction ''choochoo'' [Obj ''t'', Obj ''E'', Obj ''D''],
-  PAction ''load'' [Obj ''p1'', Obj ''D'', Obj ''t''],  
-  PAction ''choochoo'' [Obj ''t'', Obj ''D'', Obj ''E''],
-  PAction ''unload'' [Obj ''p1'', Obj ''t'', Obj ''E''],
+  SimplePlanAction STR ''drive'' [Obj STR ''c1'', Obj STR ''A'', Obj STR ''D''],
+  SimplePlanAction STR ''drive'' [Obj STR ''c1'', Obj STR ''D'', Obj STR ''C''],
+  SimplePlanAction STR ''load'' [Obj STR ''p1'', Obj STR ''C'', Obj STR ''c1''],
+  SimplePlanAction STR ''drive'' [Obj STR ''c1'', Obj STR ''C'', Obj STR ''D''],
+  SimplePlanAction STR ''unload'' [Obj STR ''p1'', Obj STR ''c1'', Obj STR ''D''],  
+  SimplePlanAction STR ''choochoo'' [Obj STR ''t'', Obj STR ''E'', Obj STR ''D''],
+  SimplePlanAction STR ''load'' [Obj STR ''p1'', Obj STR ''D'', Obj STR ''t''],  
+  SimplePlanAction STR ''choochoo'' [Obj STR ''t'', Obj STR ''D'', Obj STR ''E''],
+  SimplePlanAction STR ''unload'' [Obj STR ''p1'', Obj STR ''t'', Obj STR ''E''],
 
-  PAction ''drive'' [Obj ''c3'', Obj ''G'', Obj ''F''],
-  PAction ''load'' [Obj ''p2'', Obj ''F'', Obj ''c3''],
-  PAction ''drive'' [Obj ''c3'', Obj ''F'', Obj ''E''],
-  PAction ''unload'' [Obj ''p2'', Obj ''c3'', Obj ''E''],
+  SimplePlanAction STR ''drive'' [Obj STR ''c3'', Obj STR ''G'', Obj STR ''F''],
+  SimplePlanAction STR ''load'' [Obj STR ''p2'', Obj STR ''F'', Obj STR ''c3''],
+  SimplePlanAction STR ''drive'' [Obj STR ''c3'', Obj STR ''F'', Obj STR ''E''],
+  SimplePlanAction STR ''unload'' [Obj STR ''p2'', Obj STR ''c3'', Obj STR ''E''],
 
-  PAction ''load'' [Obj ''p1'', Obj ''E'', Obj ''c3''],
-  PAction ''drive'' [Obj ''c3'', Obj ''E'', Obj ''G''],
-  PAction ''unload'' [Obj ''p1'', Obj ''c3'', Obj ''G'']
+  SimplePlanAction STR ''load'' [Obj STR ''p1'', Obj STR ''E'', Obj STR ''c3''],
+  SimplePlanAction STR ''drive'' [Obj STR ''c3'', Obj STR ''E'', Obj STR ''G''],
+  SimplePlanAction STR ''unload'' [Obj STR ''p1'', Obj STR ''c3'', Obj STR ''G'']
 ]"
 (*
-PAction ''choochoo'' [Obj ''batmobile'', Obj ''D'', Obj ''E''],
-  PAction ''drive'' [Obj ''batmobile'', Obj ''E'', Obj ''G'']
+SimplePlanAction STR ''choochoo'' [Obj STR ''batmobile'', Obj STR ''D'', Obj STR ''E''],
+  SimplePlanAction STR ''drive'' [Obj STR ''batmobile'', Obj STR ''E'', Obj STR ''G'']
 Just taking the batmobile for a spin at the end, for fun. *)
-
+(* 
 value "enab_exec_x my_problem
-  (PAction ''drive'' [Obj ''c1'', Obj ''A'', Obj ''D'']) (set my_init)"
+  (SimplePlanAction STR ''drive'' [Obj STR ''c1'', Obj STR ''A'', Obj STR ''D'']) (set my_init)"
 
 value "valid_plan_x my_problem my_plan"
 lemma "ast_problem.valid_plan my_problem my_plan"
-  by (intro valid_plan_intro[OF wf_p1]) eval
+  by (intro valid_plan_intro[OF wf_p1]) eval *)
 
 
 subsection \<open> Type normalization \<close>
 
-
-lemma "ast_domain.restrict_dom my_domain" by eval
+(* 
+lemma "ast_domain.restrict_dom my_domain" by eval *)
 
 (* Type system shenanigans *)
 value "of_type_x my_domain (Either []) (Either [])"
-value "of_type_x my_domain (Either []) (Either [''FOO''])" (* even though FOO doesn't exist *)
-value "of_type_x my_domain (Either [''FOO'', ''BAR'']) (Either [''BAR'', ''FOO''])" (* even though both don't exist *)
-value "of_type_x my_domain (Either [''R'']) (Either [''object''])"
-
+value "of_type_x my_domain (Either []) (Either [STR ''FOO''])" (* even though FOO doesn't exist *)
+value "of_type_x my_domain (Either [STR ''FOO'', STR ''BAR'']) (Either [STR ''BAR'', STR ''FOO''])" (* even though both don't exist *)
+value "of_type_x my_domain (Either [STR ''R'']) (Either [STR ''object''])"
+(* 
 declare ast_domain.constT_def [code]
-declare ast_problem.objT_def [code]
+declare ast_problem.objT_def [code] *)
 
-value "ast_domain.is_of_type' (ast_problem.objT my_problem)
-  (ast_domain.STG my_domain) (Obj ''c1'') (Either [''Car'', ''FOO''])" (* even though FOO doesn't exist *)
+(* value "ast_domain.is_of_type' (ast_problem.objT my_problem)
+  (ast_domain.STG my_domain) (Obj STR ''c1'') (Either [STR ''Car'', STR ''FOO''])" *) (* even though FOO doesn't exist *)
 
 (* type normalization testing *)
 definition "my_type_names \<equiv> ast_domain.type_names my_domain"
 value "showvals (reachable_nodes my_types) my_type_names"
 value "ast_domain.type_preds my_domain"
 value "ast_domain.supertype_facts_for my_domain (my_objs ! 1)"
-value "ast_domain.type_precond my_domain (Var ''into'', Either [''Car'', ''Train''])"
+value "ast_domain.type_precond my_domain (Var STR ''into'', Either [STR ''Car'', STR ''Train''])"
 value "ast_domain.detype_ac my_domain op_load"
 value "detype_preds my_preds"
 
@@ -243,30 +256,30 @@ lemma wf_p4: "ast_problem.wf_problem my_prob_split"
 (* A little manual labor to decide which one of the split actions
   corresponds to which step in the original plan. *)
 definition "my_plan_3 \<equiv> [
-  PAction ''0drive'' [Obj ''c1'', Obj ''A'', Obj ''D''],
-  PAction ''1drive'' [Obj ''c1'', Obj ''D'', Obj ''C''],
-  PAction ''0load'' [Obj ''p1'', Obj ''C'', Obj ''c1''],
-  PAction ''0drive'' [Obj ''c1'', Obj ''C'', Obj ''D''],
-  PAction ''0unload'' [Obj ''p1'', Obj ''c1'', Obj ''D''],  
-  PAction ''1choochoo'' [Obj ''t'', Obj ''E'', Obj ''D''],
-  PAction ''1load'' [Obj ''p1'', Obj ''D'', Obj ''t''],  
-  PAction ''0choochoo'' [Obj ''t'', Obj ''D'', Obj ''E''],
-  PAction ''1unload'' [Obj ''p1'', Obj ''t'', Obj ''E''],
+  SimplePlanAction STR ''0drive'' [Obj STR ''c1'', Obj STR ''A'', Obj STR ''D''],
+  SimplePlanAction STR ''1drive'' [Obj STR ''c1'', Obj STR ''D'', Obj STR ''C''],
+  SimplePlanAction STR ''0load'' [Obj STR ''p1'', Obj STR ''C'', Obj STR ''c1''],
+  SimplePlanAction STR ''0drive'' [Obj STR ''c1'', Obj STR ''C'', Obj STR ''D''],
+  SimplePlanAction STR ''0unload'' [Obj STR ''p1'', Obj STR ''c1'', Obj STR ''D''],  
+  SimplePlanAction STR ''1choochoo'' [Obj STR ''t'', Obj STR ''E'', Obj STR ''D''],
+  SimplePlanAction STR ''1load'' [Obj STR ''p1'', Obj STR ''D'', Obj STR ''t''],  
+  SimplePlanAction STR ''0choochoo'' [Obj STR ''t'', Obj STR ''D'', Obj STR ''E''],
+  SimplePlanAction STR ''1unload'' [Obj STR ''p1'', Obj STR ''t'', Obj STR ''E''],
 
-  PAction ''1drive'' [Obj ''c3'', Obj ''G'', Obj ''F''],
-  PAction ''0load'' [Obj ''p2'', Obj ''F'', Obj ''c3''],
-  PAction ''1drive'' [Obj ''c3'', Obj ''F'', Obj ''E''],
-  PAction ''0unload'' [Obj ''p2'', Obj ''c3'', Obj ''E''],
+  SimplePlanAction STR ''1drive'' [Obj STR ''c3'', Obj STR ''G'', Obj STR ''F''],
+  SimplePlanAction STR ''0load'' [Obj STR ''p2'', Obj STR ''F'', Obj STR ''c3''],
+  SimplePlanAction STR ''1drive'' [Obj STR ''c3'', Obj STR ''F'', Obj STR ''E''],
+  SimplePlanAction STR ''0unload'' [Obj STR ''p2'', Obj STR ''c3'', Obj STR ''E''],
 
-  PAction ''0load'' [Obj ''p1'', Obj ''E'', Obj ''c3''],
-  PAction ''1drive'' [Obj ''c3'', Obj ''E'', Obj ''G''],
-  PAction ''0unload'' [Obj ''p1'', Obj ''c3'', Obj ''G''],
+  SimplePlanAction STR ''0load'' [Obj STR ''p1'', Obj STR ''E'', Obj STR ''c3''],
+  SimplePlanAction STR ''1drive'' [Obj STR ''c3'', Obj STR ''E'', Obj STR ''G''],
+  SimplePlanAction STR ''0unload'' [Obj STR ''p1'', Obj STR ''c3'', Obj STR ''G''],
 
-  PAction ''0Goal_____'' []
+  SimplePlanAction STR ''0Goal_____'' []
 ]"
 
-(* PAction ''choochoo'' [Obj ''batmobile'', Obj ''D'', Obj ''E''],
-  PAction ''drive'' [Obj ''batmobile'', Obj ''E'', Obj ''G''] *)
+(* SimplePlanAction STR ''choochoo'' [Obj STR ''batmobile'', Obj STR ''D'', Obj STR ''E''],
+  SimplePlanAction STR ''drive'' [Obj STR ''batmobile'', Obj STR ''E'', Obj STR ''G''] *)
 
 (* if you choose the wrong plan action at one point, this tells you where *)
 value "valid_plan_x my_prob_split my_plan_3"
@@ -308,7 +321,7 @@ definition "my_prob_reachables \<equiv> ast_problem.semi_naive_eval my_prob_rela
 value "my_prob_reachables" (* takes a minute *)
 
 value "ast_problem.all_derivs_of my_prob_relaxed
-  (as_atom ''at'' [Obj ''c1'', Obj ''A''])
+  (as_atom STR ''at'' [Obj STR ''c1'', Obj STR ''A''])
   (organize_facts (ast_problem.init' my_prob_relaxed))
   (as_action_clause (actions my_dom_relaxed ! 1))"
 
