Type_Normalization/Type_Normalization_Semantics.thy
@@ -1,0 +1,840 @@
+theory Type_Normalization_Semantics
+  imports Type_Normalization
+begin
+
+subsubsection \<open> Type Normalization Preserves Semantics \<close>
+
+context domain_signature
+begin
+
+text \<open> Supertype Facts logic \<close>
+
+  lemma of_type_iff_reach:
+    shows "of_type (Either oT) (Either T) \<longleftrightarrow> (
+      \<forall>ot \<in> set oT.
+      \<exists>t \<in> set T.
+        t \<in> set (supertypes_of ot))"
+  proof -
+    have "of_type (Either oT) (Either T) \<longleftrightarrow>
+      set oT \<subseteq> ((set ty_decl)\<^sup>*)\<inverse> `` set T"
+      using subtype_rel_star_alt of_type_def by simp
+    also have "... \<longleftrightarrow>
+      (\<forall>ot \<in> set oT. ot \<in> ((set ty_decl)\<^sup>*)\<inverse> `` set T)"
+      by auto
+    also have "... \<longleftrightarrow>
+      (\<forall>ot \<in> set oT. \<exists>t. (ot, t) \<in> (set ty_decl)\<^sup>* \<and> t \<in> set T)"
+      by auto
+    finally show ?thesis using reachable_iff_in_star describes_rel_def by metis
+  qed
+
+lemma single_of_type_iff:
+  shows "of_type (Either [ot]) (Either T) \<longleftrightarrow> (
+    \<exists>t \<in> set T.
+      t \<in> set (supertypes_of ot))"
+  using of_type_iff_reach by simp
+
+end
+context problem_signature
+begin
+
+lemma obj_of_type_iff_reach:
+  assumes "objT n = Some (Either oT)"
+  shows  "is_obj_of_type n (Either T) \<longleftrightarrow>
+    (\<forall>ot \<in> set oT.
+      \<exists>t \<in> set T.
+    t \<in> set (supertypes_of ot))"
+  using assms is_obj_of_type_def of_type_iff_reach by auto
+
+lemma type_atom_inj: "inj (type_atom n)"
+  using type_atom.simps pred_for_type_inj
+  by (simp add: inj_def)
+
+lemma simple_obj_of_type_iff:
+  assumes "objT n = Some (Either [ot])"
+  shows  "is_obj_of_type n (Either T) \<longleftrightarrow>
+      (\<exists>t \<in> set T.
+    t \<in> set (supertypes_of ot))"
+  using assms is_obj_of_type_def single_of_type_iff by auto
+
+lemma simple_obj_of_type_iff_fact:
+  assumes "objT n = Some oT" "single_type oT"
+  shows "is_obj_of_type n (Either T) \<longleftrightarrow>
+    (\<exists>t \<in> set T.
+    (type_atom n t) \<in> set (supertype_facts_for (n, oT)))"
+proof -
+  from assms(2) obtain ot where [simp]: "oT = Either [ot]"
+    by (auto intro: type_decomp_1)
+  hence "is_obj_of_type n (Either T) \<longleftrightarrow>
+    (\<exists>t \<in> set T.
+    (type_atom n t) \<in> (type_atom n) ` set (supertypes_of ot))"
+    using assms simple_obj_of_type_iff type_atom_inj inj_image_mem_iff by metis
+  thus ?thesis using assms(1) by simp
+qed
+end
+
+
+context wf_restrict_problem_signature
+begin
+lemma (in restrict_problem_signature2) sf_basic: "lwm_basic sf_substate"
+  unfolding lwm_basic_def 
+  using supertype_facts_predAtom by argo
+
+lemma typeatm_iff_obj_listed:
+  assumes "type_atom n t \<in> sf_substate"
+  obtains oT where "(n, oT) \<in> set (all_consts)"
+  using assms supertype_facts_def superfacts_for_cond single_t_consts by fastforce
+
+theorem obj_of_type_iff_typeatom:
+  shows "is_obj_of_type n (Either T) \<longleftrightarrow>
+    (\<exists>t \<in> set T.
+     type_atom n t \<in> sf_substate)" (is "?L \<longleftrightarrow> ?R")
+proof
+  assume L: ?L
+  moreover obtain oT where ot: "(n, oT) \<in> set (all_consts)"
+    using L objT_Some is_obj_of_type_def by (cases "objT n"; simp)
+  moreover have "set (supertype_facts_for (n, oT)) \<subseteq> sf_substate"
+    using supertype_facts_def ot by auto
+  ultimately show ?R
+    using simple_obj_of_type_iff_fact single_t_consts objT_Some
+    by (metis case_prod_conv subset_code(1))
+next
+  assume R: ?R
+  then obtain oT where ot: "(n, oT) \<in> set (all_consts)"
+    using typeatm_iff_obj_listed by auto
+  from R  obtain t where tin: "t \<in> set T" and "type_atom n t \<in> sf_substate" ..
+  then obtain n' T' where
+    1: "type_atom n t \<in> set (supertype_facts_for (n', T'))" and
+    2: "(n', T') \<in> set (all_consts)"
+    using supertype_facts_def by auto
+  from 2 have "single_type T'" using single_t_consts by auto
+  hence "n = n'" using 1 superfacts_for_cond by auto
+  moreover hence "oT = T'" using 2 ot
+    by (metis objT_Some option.inject)
+  ultimately have "type_atom n t \<in> set (supertype_facts_for (n, oT))" using 1 by simp
+  thus ?L
+    using ot objT_Some single_t_consts tin simple_obj_of_type_iff_fact by blast
+qed
+
+theorem obj_of_type_iff2:
+  assumes "wf_type (Either T)"
+  shows "is_obj_of_type n (Either T) \<longleftrightarrow> valuation (sf_substate, x) \<Turnstile>\<^sub>m \<^bold>\<Or>(map (type_atom n) T)"
+proof -
+  have "is_obj_of_type n (Either T) \<longleftrightarrow>
+    (\<exists>t \<in> set T. valuation (sf_substate, x) \<Turnstile>\<^sub>m type_atom n t)"
+    using obj_of_type_iff_typeatom valuation_def by simp
+  also have "... \<longleftrightarrow> valuation (sf_substate, x) \<Turnstile>\<^sub>m \<^bold>\<Or>(map (type_atom n) T)"
+  proof -
+    have "\<forall>f \<in> set (map (type_atom n) T). atoms f \<subseteq> dom (valuation (sf_substate, x))"
+      by auto
+    thus ?thesis by auto
+  qed
+  finally show ?thesis by auto
+qed
+
+lemma obj_of_vartype_iff:
+  assumes "subst_term f (term.VAR v) = n"
+      and "wf_type vT"
+  shows "is_obj_of_type n vT \<longleftrightarrow>
+    valuation (sf_substate, x) \<Turnstile>\<^sub>m map_atom_fmla (subst_term f) (type_precond (v, vT))"
+proof -
+  let ?map_subst = "map_atom_fmla (subst_term f)"
+  have 1: "map (type_atom n) (primitives vT) = map (?map_subst \<circ> type_atom (term.VAR v)) (primitives vT)"
+    using assms by simp
+  have 2: "\<^bold>\<Or>(map (?map_subst \<circ> (type_atom (term.VAR v))) (primitives vT))
+    = ?map_subst \<^bold>\<Or>(map ((type_atom (term.VAR v))) (primitives vT))"
+    using map_formula_bigOr by (metis comp_apply list.map_comp)
+  have "is_obj_of_type n vT \<longleftrightarrow> valuation (sf_substate, x) \<Turnstile>\<^sub>m \<^bold>\<Or>(map (type_atom n) (primitives vT))"
+    using obj_of_type_iff2 assms(2) by (cases vT) force
+  thus ?thesis using 1 2 type_precond.simps
+    by (metis type.exhaust_sel)
+qed
+
+lemma obj_of_vartype_iff2:
+  assumes a:
+    "distinct (map fst params)"
+    "params ! i = (v, vT)" "args ! i = n"
+    "i < length params" "i < length args"
+  and wf: "wf_type vT"
+  shows "is_obj_of_type n vT \<longleftrightarrow>
+    valuation (sf_substate, x) \<Turnstile>\<^sub>m map_atom_fmla (ac_tsubst params args) (type_precond (v, vT))"
+  using ac_tsubst_intro assms obj_of_vartype_iff by simp
+
+(* using this logic for the next lemma *)
+lemma "(b \<Longrightarrow> (c \<longleftrightarrow> d)) \<Longrightarrow> b \<and> c \<longleftrightarrow> b \<and> d" by auto
+
+(* forgive me, father, for I have sinned; TODO: simplify *)
+theorem (in restrict_classical_problem2) params_match_iff_type_precond:
+  assumes "wf_classical_action_schema ac"
+  assumes "wf_action_params ac"
+  defines "params \<equiv> ac_params ac"
+  defines "h \<equiv> ac_head ac"
+  shows "action_params_match h args \<longleftrightarrow>
+    length params = length args \<and>
+    valuation (sf_substate, x) \<Turnstile>\<^sub>m map_atom_fmla (ac_tsubst params args) (param_precond params)"
+proof -
+  let ?leq = "length params = length args"
+  define el_map where "el_map \<equiv> map_atom_fmla (ac_tsubst params args)"
+
+  have dis: "distinct (map fst params)" using assms wf_classical_action_schema_alt by metis
+
+  have 1: "action_params_match h args \<longleftrightarrow>
+    ?leq \<and>
+    (\<forall>i < (length params). is_obj_of_type (args ! i) (snd (params ! i)))"
+    unfolding params_def h_def action_params_match_def list_all2_conv_all_nth
+    by force
+  {
+    assume ?leq
+    {
+      fix i assume l: "i < length params"
+
+      obtain v vT where
+        pi: "params ! i = (v, vT)" using l apply (cases "params ! i") by auto
+
+      have "params ! i \<in> set (ac_params ac)" using l params_def by simp
+      hence wft: "wf_type vT" using assms wf_action_params_def pi by auto
+      
+      have "is_obj_of_type (args ! i) (snd (params ! i))
+      \<longleftrightarrow> valuation (sf_substate, x) \<Turnstile>\<^sub>m  el_map (type_precond (params ! i))"
+        unfolding el_map_def pi
+        apply (subst obj_of_vartype_iff2[symmetric])
+        using dis \<open>?leq\<close> assms l pi wft
+        unfolding is_obj_of_type_def el_map_def snd_conv by simp_all
+    }
+    hence "(\<forall>i < length params. is_obj_of_type (args ! i) (snd (params ! i))) \<longleftrightarrow>
+      (\<forall>\<phi> \<in> {el_map (type_precond (params ! i)) | i. i < length params}. valuation (sf_substate, x) \<Turnstile>\<^sub>m  \<phi>)"
+      by blast
+    also have "... \<longleftrightarrow>
+      (\<forall>\<phi> \<in> set (map (el_map \<circ> type_precond) params). valuation (sf_substate, x) \<Turnstile>\<^sub>m  \<phi>)"
+      using map_set_comprehension[where f="el_map \<circ> type_precond"] by fastforce
+    also have "... \<longleftrightarrow> valuation (sf_substate, x) \<Turnstile>\<^sub>m  \<^bold>\<And>(map (el_map \<circ> type_precond) params)"
+      using BigAnd_map_semantics by blast
+    also have "... \<longleftrightarrow> valuation (sf_substate, x) \<Turnstile>\<^sub>m  el_map (\<^bold>\<And>(map type_precond params))"
+      by (simp add: bigAnd_map_atom[simplified comp_def, symmetric] comp_def el_map_def)
+    note calculation
+  }
+  thus ?thesis using 1 el_map_def bigAnd_map_atom
+    by (metis (no_types, opaque_lifting) map_map param_precond_def)
+qed
+
+end
+
+
+(* INSTANTIATE STUFF *)
+
+lemma (in restrict_classical_problem2) t_resinst:
+  assumes "resolve_classical_action_schema n = Some ac"
+  shows "d2.resolve_classical_action_schema n = Some (detype_classical_ac ac)"
+proof -
+  from assms have a: "ac \<in> set (actions D)"
+    by (metis index_by_eq_SomeD resolve_classical_action_schema_def)
+  from assms have b: "ac_name ac = n"
+    by (metis resolve_classical_action_schema_def index_by_eq_SomeD)
+  hence "ac_name (detype_classical_ac ac) = n" by simp
+  moreover have "detype_classical_ac ac \<in> set (actions D2)"
+    using a by auto
+  ultimately show ?thesis using wf_D
+    by (simp add: d2.resolve_classical_action_schema_def)
+qed
+
+lemma (in restrict_classical_problem2) t_resinst_inv:
+  assumes "p2.resolve_classical_action_schema n = Some ac2"
+  obtains ac where
+    "detype_classical_ac ac = ac2"
+    "ac \<in> set (actions D)"
+    "resolve_classical_action_schema n = Some ac"
+proof -
+  from assms obtain ac where ac: "detype_classical_ac ac = ac2" and ac_in: "ac \<in> set (actions D)"
+    using res_aux by auto
+  hence "ac_name (detype_classical_ac ac) = n"
+    using p2.resolve_classical_action_schema_def index_by_eq_SomeD assms by metis
+  hence "ac_name ac = n" by simp
+  thus ?thesis using that ac ac_in resolve_classical_action_schema_def wf_DP
+    by simp
+qed
+
+subsubsection \<open> Semantics \<close>
+
+
+text \<open> Type atom/Supertype facts inclusion/exclusion/overlap \<close>
+(* TODO: reevaluate what is necessary, maybe use fmla_preds in proofs *)
+
+context ast_classical_domain begin
+lemma wf_patm_neq_type_patm:
+  assumes "wf_pred_atom tyt (p, xs)"
+  shows "type_predatm x t \<noteq> map_atom f (predAtm p xs)"
+proof -
+  from assms have "p \<in> pred ` set (predicates D)"
+    using sig_None wf_pred_atom.simps by (metis option.simps(4))
+  thus ?thesis using type_pred_notin by auto
+qed
+
+lemma wf_fmla_atom_neq_type_atom:
+  assumes "wf_fmla_atom tyt \<phi>"
+  shows "map_atom_fmla f \<phi> \<noteq> type_atom x t"
+  using assms apply (cases rule: wf_fmla_atom.cases[of \<phi>])
+  using wf_patm_neq_type_patm by fastforce+
+
+(*lemma wf_fmla_atom_neq_type_atom_unatm:
+  assumes "wf_fmla_atom tyt \<phi>"
+  shows "un_Atom (map_atom_fmla f \<phi>) \<noteq> type_predatm x t"
+  using assms apply (cases rule: wf_fmla_atom.cases[of \<phi>])
+  using wf_patm_neq_type_patm by fastforce+*)
+
+lemma wf_fmla_no_type_patms:
+  assumes "wf_fmla tyt \<phi>"
+  shows "type_predatm n t \<notin> atoms (map_atom_fmla f \<phi>)"
+proof -
+  have "atoms (map_atom_fmla f \<phi>) = (map_atom f) ` (atoms \<phi>)"
+    by (simp add: formula.set_map)
+  moreover have "type_predatm n t \<notin> (map_atom f) ` (atoms \<phi>)"
+  using assms proof (induction \<phi>)
+    case (Atom a)
+    thus ?case
+    proof (cases a)
+      case (predAtm p vs)
+      thus ?thesis using wf_patm_neq_type_patm Atom predAtm by fastforce
+    qed auto (* Obviously, type_predatm n t \<noteq> Eq a b. *)
+  qed auto
+  ultimately show ?thesis by simp
+qed
+
+lemma (in restrict_classical_problem) sf_typeatms:
+  assumes "\<psi> \<in> sf_substate"
+  shows "\<exists>n t. \<psi> = type_atom n t"
+  using assms superfacts_unfolded by auto
+
+lemma (in restrict_classical_problem) sf_disj_wf_fmla:
+  assumes "wf_fmla tyt \<phi>"
+  shows "sf_substate \<inter> Atom ` atoms (map_atom_fmla f \<phi>) = {}"
+  using assms sf_typeatms wf_fmla_no_type_patms by fastforce
+
+lemma fmla_map_id: "map_atom_fmla id \<phi> = \<phi>"
+  by (simp add: atom.map_id0 formula.map_id)
+
+lemma (in restrict_classical_problem) sf_disj_wf_fmla0:
+  assumes "wf_fmla tyt \<phi>"
+  shows "sf_substate \<inter> Atom ` atoms \<phi> = {}"
+  using assms sf_disj_wf_fmla[where f=id] fmla_map_id by metis
+
+lemma (in -) "map_ast_effect f (Effect A D N) =
+  Effect (map (map_atom_fmla f) A) (map (map_atom_fmla f) D) (map (map_numeric_effect f) N)"
+  by simp
+
+lemma wf_eff_no_type_atoms:
+  assumes "wf_effect tyt \<epsilon>"
+  shows
+    "type_atom n t \<notin> set (adds (map_ast_effect f \<epsilon>))" (is ?a) and
+    "type_atom n t \<notin> set (dels (map_ast_effect f \<epsilon>))" (is ?d)
+proof -
+  from assms have "\<forall>\<phi> \<in> set (adds \<epsilon>). wf_fmla_atom tyt \<phi>"
+    using assms by (cases \<epsilon>) simp
+  hence "\<forall>\<phi> \<in> (map_atom_fmla f) ` set (adds \<epsilon>). \<phi> \<noteq> type_atom n t"
+    using wf_fmla_atom_neq_type_atom by fast
+  thus ?a by (cases \<epsilon>) auto
+
+  from assms have "\<forall>\<phi> \<in> set (dels \<epsilon>). wf_fmla_atom tyt \<phi>"
+    using assms by (cases \<epsilon>) simp
+  hence "\<forall>\<phi> \<in>(map_atom_fmla f) ` set (dels \<epsilon>). \<phi> \<noteq> type_atom n t"
+    using wf_fmla_atom_neq_type_atom by fast
+  thus ?d by (cases \<epsilon>) auto
+qed
+
+
+abbreviation "is_type_patm a \<equiv> \<exists>x t. a = type_predatm x t"
+
+
+lemma map_atom_preserves_istypeatm: "is_type_patm a \<longleftrightarrow> is_type_patm (map_atom f a)"
+  by (cases a) auto
+
+lemma map_fmla_preserves_istypeatm:
+  assumes "\<forall>a \<in> atoms F. is_type_patm a"
+  shows "\<forall>a \<in> atoms (map_atom_fmla f F). is_type_patm a"
+proof -
+  have "atoms (map_atom_fmla f F) = (map_atom f) ` (atoms F)"
+    by (simp add: formula.set_map)
+  thus ?thesis using assms
+    apply (induction F)
+    apply simp_all
+       apply (metis map_atom_preserves_istypeatm)+
+    done
+qed
+
+lemma map_fmla_preserves_nistypeatm:
+  assumes "\<forall>a \<in> atoms F. \<not> is_type_patm a"
+  shows "\<forall>a \<in> atoms (map_atom_fmla f F). \<not> is_type_patm a"
+proof -
+  have "atoms (map_atom_fmla f F) = (map_atom f) ` (atoms F)"
+    by (simp add: formula.set_map)
+  thus ?thesis using assms
+    apply (induction F)
+    apply simp_all
+       apply (metis map_atom_preserves_istypeatm)+
+    done
+qed
+
+lemma param_pre_typeatms:
+  "\<forall> a \<in> atoms (map_atom_fmla f (param_precond params)). \<exists>x t. a = type_predatm x t"
+proof -
+  let ?is_typatm = "\<lambda>a. (\<exists>x t. a = type_predatm x t)"
+  have "\<forall> f \<in> set (map (type_atom (term.VAR v)) ts).
+    \<forall>a \<in> atoms f. \<exists>x t. a = type_predatm x t" for v ts by auto
+  hence "\<forall>a \<in> atoms (type_precond (v, (Either ts))). \<exists>x t. a = type_predatm x t"
+    for v ts
+    by (induction ts) auto
+  hence "\<forall>a \<in> atoms (type_precond param). \<exists>x t. a = type_predatm x t" for param
+    by (cases rule: type_precond.cases[of param]) simp
+  hence "\<forall> f \<in> set (map type_precond params).
+    \<forall>a \<in> atoms f. \<exists>x t. a = type_predatm x t" by simp
+  hence "\<forall> a \<in> atoms (param_precond params). \<exists>x t. a = type_predatm x t"
+    unfolding param_precond_def by (induction params) auto
+  with map_fmla_preserves_istypeatm show ?thesis by blast
+qed
+
+lemma (in ast_classical_problem) wf_wm_no_typeatms:
+  "wf_world_model wm \<Longrightarrow> type_atom x t \<notin> fst wm"
+  using wf_fmla_atom_neq_type_atom by (cases wm) fastforce
+
+lemma (in ast_classical_problem) wf_wm_disj_param_pre:
+  assumes "wf_world_model wm"
+  shows "fst wm \<inter> Atom ` atoms (map_atom_fmla f (param_precond params)) = {}"
+  using assms wf_wm_no_typeatms param_pre_typeatms by (cases wm) force
+
+(* for wf init, since sf and init don't overlap *)
+lemma (in restrict_classical_problem) sf_disj_wf_wm:
+  assumes "wf_world_model wm"
+  shows "sf_substate \<inter> fst wm = {}"
+proof -
+  from assms have "\<forall>\<phi> \<in> fst wm. wf_fmla_atom objT \<phi>" by (cases wm) force
+  hence "type_atom x t \<notin> fst wm" for x t
+    using wf_fmla_atom_neq_type_atom by fastforce
+  thus ?thesis using sf_typeatms by blast
+qed
+
+lemma (in restrict_classical_problem) sf_disj_wf_eff:
+  assumes "wf_effect tyt \<epsilon>"
+  shows
+    "sf_substate \<inter> set (adds (map_ast_effect f \<epsilon>)) = {}"
+    "sf_substate \<inter> set (dels (map_ast_effect f \<epsilon>)) = {}"
+  using assms sf_typeatms wf_eff_no_type_atoms by fast+
+
+lemmas in_ex_clusion_helpers =
+  wf_patm_neq_type_patm
+  wf_fmla_no_type_patms
+
+end
+
+(* All of these could maybe be intelligently moved somewhere else... *)
+hide_fact
+  ast_classical_domain.wf_patm_neq_type_patm
+  ast_classical_domain.wf_fmla_no_type_patms
+  restrict_classical_problem.sf_typeatms
+  ast_classical_domain.wf_fmla_atom_neq_type_atom
+  ast_classical_problem.wf_wm_no_typeatms
+  ast_classical_domain.param_pre_typeatms
+  ast_classical_domain.map_atom_preserves_istypeatm
+  ast_classical_domain.map_fmla_preserves_istypeatm
+  ast_classical_domain.map_fmla_preserves_nistypeatm
+  (* ast_classical_domain.wf_fmla_atom_neq_type_atom_unatm *)
+
+(* ------ end inclusion/exclusion *)
+
+context restrict_classical_problem2
+begin
+
+lemma t_params_match:
+  assumes "action_params_match (ac_head ac) args"
+  shows "p2.action_params_match (head (detype_classical_ac ac)) args"
+proof -
+  from assms have len: "length (ac_params ac) = length args"
+    by (simp add: list_all2_lengthD action_params_match_def)
+  hence len2: "length (ac_params (detype_classical_ac ac)) = length args"
+    apply (cases ac rule: ast_classical_action_schema_cases_unfold)
+    by (simp add: detype_ents_def)
+
+  have "p2.is_obj_of_type (args ! i) (snd (ac_params (detype_classical_ac ac) ! i))"
+    if "i < length args" for i
+  proof -
+    have "is_obj_of_type (args ! i) (snd ((ac_params ac) ! i))"
+      using that assms len
+      by (simp add: action_params_match_def list_all2_conv_all_nth)
+    hence "objT (args ! i) \<noteq> None" using is_obj_of_type_def by (metis option.simps(4))
+    hence "p2.is_obj_of_type (args ! i) \<omega>" using t_objT_Some p2.is_obj_of_type_def by simp
+    thus ?thesis using that len2 by (simp add: detype_ent_alt detype_ents_def)
+  qed
+  thus "?thesis"
+    by (simp add: len2 list_all2_conv_all_nth p2.action_params_match_def del: detype_classical_ac_sel)
+qed
+end
+
+
+context restrict_classical_problem2
+begin
+(* TODO clean this up, if possible *)
+theorem detyped_planaction_enabled_iff:
+  assumes "wf_world_model s"
+  shows "plan_action_enabled \<pi> s \<longleftrightarrow> p2.plan_action_enabled \<pi> (s \<union> sf_substate)"
+proof -
+  obtain n args where pi: "\<pi> = PAction n args" by (cases \<pi>; simp)
+  let ?pi = "PAction n args"
+
+  from assms have s_basic: "wm_basic s" using wf_wm_basic by simp
+
+  {
+    assume assm: "plan_action_enabled ?pi s"
+    hence wf: "wf_plan_action ?pi" and entail: "s \<^sup>c\<TTurnstile>\<^sub>= precondition (resolve_instantiate ?pi)"
+      using plan_action_enabled_def by simp_all
+
+    (* actions *)
+    from wf obtain ac where res: "resolve_action_schema n = Some ac"
+      by fastforce
+    hence res2: "d2.resolve_action_schema n = Some (detype_classical_ac ac)"
+      by (rule t_resinst)
+
+    (* parameter mappings *)
+    let ?pre_map = "map_atom_fmla (ac_tsubst (parameters ac) args)"
+    let ?pre_map2 = "map_atom_fmla (ac_tsubst (parameters (detype_classical_ac ac)) args)"
+    have "map fst (parameters (detype_classical_ac ac)) = map fst (parameters ac)"
+      by (cases ac; simp add: t_ents_names)
+    hence premaps: "?pre_map2 = ?pre_map" using ac_tsubst_def by simp
+
+    (* "left" side: from wf_plan_action \<pi> show p2.wf_plan_action \<pi> *)
+    from wf res have match: "action_params_match ac args" by simp
+    hence "p2.action_params_match (detype_classical_ac ac) args"
+      using t_params_match by simp
+    with res2 have wf2: "p2.wf_plan_action ?pi"
+      using p2.wf_plan_action_simple by fastforce
+
+    (* "middle": from action_params_match ac args show s \<union> sf_substate satisfy the param precond of the instantiated action.*)
+    from match have entail_typ: "sf_substate \<^sup>c\<TTurnstile>\<^sub>= ?pre_map (param_precond (ac_params ac))"
+      using params_match_iff_type_precond res res_aux wf_D(7) by simp
+    (* Since init doesn't interfere with the type predicates,
+       we can add it to sf_substate here and still satisfy them. *)
+    from assms have "s \<inter> Atom ` atoms (?pre_map (param_precond (ac_params ac))) = {}"
+      using wf_wm_disj_param_pre by simp
+    with entail_typ have entail_L: "s \<union> sf_substate \<^sup>c\<TTurnstile>\<^sub>= ?pre_map (param_precond (ac_params ac))"
+      using entail_adds_irrelevant[OF sf_basic s_basic] Un_commute by metis
+    
+    (* "right" side: show s satisfies action precond \<Longrightarrow> s \<union> sf_substate satisfies instantiated action precond in P2 *)
+    have entail_pre: "s \<^sup>c\<TTurnstile>\<^sub>= ?pre_map (ac_pre ac)"
+      using entail res instantiate_action_schema_alt by force
+    (* Since sf_substate doesn't interfere with the precondition,
+       we can add it to init here and still satisfy it. *)
+    have "wf_classical_action_schema ac" using res wf_D(7) res_aux by simp
+    hence "wf_fmla (ty_term (map_of (ac_params ac)) constT) (ac_pre ac)"
+      using wf_classical_action_schema_alt by simp
+    hence "sf_substate \<inter> Atom ` atoms (?pre_map (ac_pre ac)) = {}"
+      using sf_disj_wf_fmla by blast
+    with entail_pre have entail_R: "s \<union> sf_substate \<^sup>c\<TTurnstile>\<^sub>= ?pre_map (ac_pre ac)"
+      using entail_adds_irrelevant[OF s_basic sf_basic] by simp
+
+    (* putting it together *)
+    from entail_L entail_R have entail_map2:
+      "s \<union> sf_substate \<^sup>c\<TTurnstile>\<^sub>= ?pre_map2 ((param_precond (ac_params ac)) \<^bold>\<and> (ac_pre ac))"
+      using entail_and premaps by auto
+    hence entail2: "s \<union> sf_substate \<^sup>c\<TTurnstile>\<^sub>= precondition (p2.resolve_instantiate ?pi)"
+      using entail_map2 res2 by (simp add: p2.instantiate_action_schema_alt)
+    with wf2 have "p2.plan_action_enabled ?pi (s \<union> sf_substate)"
+      by (simp add: p2.plan_action_enabled_def)
+  }
+  moreover {
+    assume "p2.plan_action_enabled ?pi (s \<union> sf_substate)"
+    hence wf2: "p2.wf_plan_action ?pi" and entail2: "s \<union> sf_substate \<^sup>c\<TTurnstile>\<^sub>= precondition (p2.resolve_instantiate ?pi)"
+      using p2.plan_action_enabled_def by simp_all
+
+    (* actions *)
+    from wf2 obtain ac2 where res2: "p2.resolve_action_schema n = Some ac2"
+      using p2.wf_pa_refs_ac by metis
+    then obtain ac where ac[simp]: "ac2 = detype_classical_ac ac" and ac_in: "ac \<in> set (actions D)"
+      and res: "resolve_action_schema n = Some ac" by (metis t_resinst_inv)
+
+    (* parameter mappings *)
+    let ?pre_map2 = "map_atom_fmla (ac_tsubst (ac_params ac2) args)"
+    let ?pre_map = "map_atom_fmla (ac_tsubst (ac_params ac) args)"
+    have t_param_names: "map fst (parameters ac) = map fst (parameters (detype_classical_ac ac))"
+      by (cases ac; simp add: t_ents_names)
+    hence premaps: "?pre_map = ?pre_map2" using ac_tsubst_def by simp
+
+    (* "right" side *)
+    have "s \<union> sf_substate \<^sup>c\<TTurnstile>\<^sub>= ?pre_map2 (ac_pre ac2)"
+      using entail2 res2 instantiate_action_schema_alt by force
+    hence entail2: "s \<union> sf_substate \<^sup>c\<TTurnstile>\<^sub>= ?pre_map (param_precond (ac_params ac)) \<^bold>\<and> ?pre_map (ac_pre ac)"
+      using premaps by force
+    hence entail_a: "s \<union> sf_substate \<^sup>c\<TTurnstile>\<^sub>= ?pre_map (ac_pre ac)"
+      using entail_and by blast
+    (* Since sf_substate doesn't interfere with the precondition,
+       we can remove it from init here and still satisfy it. *)
+    from ac_in have wf_ac: "wf_classical_action_schema ac" using wf_D(7) by simp
+    hence "wf_fmla (ty_term (map_of (ac_params ac)) constT) (ac_pre ac)"
+      using wf_classical_action_schema_alt by simp
+    hence "sf_substate \<inter> Atom ` atoms (?pre_map (ac_pre ac)) = {}"
+      using sf_disj_wf_fmla by simp
+    with entail_a have "s \<^sup>c\<TTurnstile>\<^sub>= ?pre_map (ac_pre ac)"
+      using entail_adds_irrelevant[OF s_basic sf_basic] by simp
+    hence entail: "s \<^sup>c\<TTurnstile>\<^sub>= precondition (resolve_instantiate ?pi)"
+      using res instantiate_action_schema_alt by simp
+
+    (* "middle" *)
+    from wf2 res2 have match2: "p2.action_params_match ac2 args" by simp
+    (* Since init doesn't interfere with the type predicates,
+       we can remove it from i2 here and still satisfy them. *)
+    have "\<forall>\<phi> \<in> s. wf_fmla_atom objT \<phi>"
+      using assms wf_fmla_atom_alt wf_world_model_def by simp
+    from assms have "s \<inter> Atom ` atoms (?pre_map (param_precond (ac_params ac))) = {}"
+      using wf_wm_disj_param_pre by simp
+    moreover from entail2 have "s \<union> sf_substate \<^sup>c\<TTurnstile>\<^sub>= ?pre_map (param_precond (ac_params ac))"
+      using entailment_def entail_and by blast
+    ultimately have entail_typ: "sf_substate \<^sup>c\<TTurnstile>\<^sub>= ?pre_map (param_precond (ac_params ac))"
+      using entail_adds_irrelevant[OF sf_basic s_basic] by (simp add: Set.Un_commute)
+
+    (* "left" side *)
+    hence "length (ac_params ac2) = length args"
+      using match2 p2.action_params_match_def by (simp add: list_all2_lengthD)
+    moreover have "length (ac_params ac) = length (ac_params (detype_classical_ac ac))"
+      using t_param_names map_eq_imp_length_eq by blast (*weird way to prove this*)
+    ultimately have "length (ac_params ac) = length args"
+      using detype_ents_def by simp
+    hence "action_params_match ac args"
+      using params_match_iff_type_precond[OF wf_ac] entail_typ by simp
+    with res have wf: "wf_plan_action ?pi" using wf_plan_action_simple by fastforce
+
+    from entail wf have "plan_action_enabled ?pi s"
+      by (simp add: plan_action_enabled_def)
+  }
+  ultimately show ?thesis using pi by auto
+qed
+
+abbreviation "states_match s s' \<equiv> wf_world_model s \<and> s \<union> sf_substate = s'"
+
+lemma match_state_step:
+  assumes "states_match s s'" "execute_plan_action \<pi> s = t" "wf_plan_action \<pi>"
+  shows "states_match t (p2.execute_plan_action \<pi> s')"
+proof -
+  obtain n args where pi: "\<pi> = PAction n args" by (cases \<pi>) simp
+  then obtain ac where res: "resolve_action_schema n = Some ac"
+    using assms(3) plan_action_enabled_def by fastforce
+  hence 1: "effect (resolve_instantiate \<pi>) = map_ast_effect (ac_tsubst (ac_params ac) args) (ac_eff ac)"
+    using pi instantiate_action_schema_alt by simp
+
+  from pi obtain ac2 where res2: "p2.resolve_action_schema n = Some ac2" and t_ac: "ac2 = detype_classical_ac ac"
+    using res t_resinst by simp
+  hence 2: "effect (p2.resolve_instantiate \<pi>) = map_ast_effect (ac_tsubst (ac_params ac2) args) (ac_eff ac2)"
+    using pi instantiate_action_schema_alt by simp
+
+  from t_ac have "map fst (ac_params ac) = map fst (ac_params ac2)"
+    by (simp add: t_ents_names)
+  moreover from t_ac have "ac_eff ac = ac_eff ac2" by simp
+  ultimately have effeq: "effect (resolve_instantiate \<pi>) = effect (p2.resolve_instantiate \<pi>)"
+    using ac_tsubst_def 1 2 by force
+
+  note wf_resolve_instantiate[OF assms(3)]
+  hence "wf_effect objT (effect (resolve_instantiate \<pi>))"
+    by (simp add: wf_ground_action_alt)
+  with sf_disj_wf_eff[OF this, where f = id] have
+    "sf_substate \<inter> set (adds (effect (resolve_instantiate \<pi>))) = {}"
+    "sf_substate \<inter> set (dels (effect (resolve_instantiate \<pi>))) = {}"
+    by (simp_all add: ast_effect.map_id)
+
+  hence "apply_effect (effect (resolve_instantiate \<pi>)) (s \<union> sf_substate) =
+    apply_effect (effect (resolve_instantiate \<pi>)) s \<union> sf_substate"
+    using 1 apply_effect_alt sf_disj_wf_wm by auto
+  hence "p2.execute_plan_action \<pi> s' = execute_plan_action \<pi> s \<union> sf_substate"
+    using effeq execute_plan_action_def
+    using p2.execute_plan_action_def assms(1) by simp
+  moreover have "wf_world_model (execute_plan_action \<pi> s)" using wf_execute_stronger assms by auto
+  ultimately show ?thesis using assms(2) by simp
+qed
+
+lemma goal_sem:
+  assumes "wm_basic s"
+  shows "s \<^sup>c\<TTurnstile>\<^sub>= goal P \<longleftrightarrow> s \<union> sf_substate \<^sup>c\<TTurnstile>\<^sub>= goal P2"
+proof -  
+  have 1: "s \<^sup>c\<TTurnstile>\<^sub>= goal P \<longleftrightarrow> s \<^sup>c\<TTurnstile>\<^sub>= goal P2" by simp
+  have c3: "sf_substate \<inter> Atom ` atoms (goal P2) = {}"
+    using detype_classical_prob_sel(4) fmla_map_id sf_disj_wf_fmla[where f = id] wf_P(5) by metis
+  note entail_adds_irrelevant[OF assms sf_basic c3]
+  with 1 show ?thesis by simp
+qed
+lemma match_goal:
+  assumes "states_match s s'"
+  shows "s \<^sup>c\<TTurnstile>\<^sub>= goal P \<longleftrightarrow> s' \<^sup>c\<TTurnstile>\<^sub>= goal P2"
+  using assms goal_sem wf_wm_basic by simp
+
+lemma match_valid_classical_plan_from2:
+  assumes "states_match s s'" "valid_classical_plan_from2 s \<pi>s"
+  shows "p2.valid_classical_plan_from2 s' \<pi>s"
+using assms proof (induction \<pi>s arbitrary: s s')
+  case Nil
+  hence "s \<^sup>c\<TTurnstile>\<^sub>= goal P"
+    using valid_classical_plan_from2_def by simp
+  hence "s' \<^sup>c\<TTurnstile>\<^sub>= goal P2" using assms match_goal Nil.prems by simp
+  thus ?case using p2.valid_classical_plan_from2_def by auto
+next
+  case (Cons p ps)
+  let ?t = "execute_plan_action p s"
+  let ?t' = "p2.execute_plan_action p s'"
+  from Cons have enab1: "plan_action_enabled p s" and valid1: "valid_classical_plan_from2 ?t ps"
+    using valid_classical_plan_from2_def plan_action_path_Cons by auto
+  from enab1 have enab2: "p2.plan_action_enabled p s'"
+    using detyped_planaction_enabled_iff assms(1) Cons.prems by simp
+  
+  have "states_match ?t ?t'"
+    using assms(1) enab1 Cons.prems match_state_step plan_action_enabled_def
+    by blast
+
+  hence "p2.valid_classical_plan_from2 ?t' ps"
+    using Cons.IH[OF _ valid1] by simp
+  with enab2 show ?case using p2.valid_classical_plan_from2_def plan_action_path_Cons by simp
+qed
+
+lemma inits_match:
+  shows "states_match I p2.I" using wf_I by auto
+
+lemma match_valid_classical_plan:
+  assumes "valid_classical_plan \<pi>s" shows "p2.valid_classical_plan \<pi>s"
+  using assms unfolding ast_classical_problem.valid_classical_plan_def
+  using match_valid_classical_plan_from2 inits_match by blast
+
+text \<open>Proving: p2.valid_classical_plan \<pi>s \<Longrightarrow> valid_classical_plan \<pi>s \<close>
+
+
+abbreviation reachable_prop :: "world_model \<Rightarrow> bool" where
+  "reachable_prop s' \<equiv> \<exists>s. states_match s s'"
+abbreviation (input) "RP \<equiv> reachable_prop"
+
+lemma rp_props:
+  assumes "RP M"
+  shows
+    "p2.wf_world_model M"
+    "\<forall>x t. type_atom x t \<in> M \<longleftrightarrow> type_atom x t \<in> sf_substate"
+    "wf_world_model (M - sf_substate)"
+proof -
+  from assms show "p2.wf_world_model M" using t_wm_wf
+    using p2.wf_world_model_def super_facts_wf by auto
+  (* if problem: super_facts_wf might need wf_wm_def *)
+  from assms show "\<forall>x t. type_atom x t \<in> M \<longleftrightarrow> type_atom x t \<in> sf_substate"
+    using wf_wm_no_typeatms by force
+  from assms obtain s where "states_match s M" by blast
+  thus "wf_world_model (M - sf_substate)"
+    using wf_world_model_def by auto
+qed
+
+lemma rp_init: "RP p2.I"
+proof -
+  have "p2.I = I \<union> sf_substate" by auto
+  thus ?thesis using wf_P(4) by auto
+qed
+
+lemma rp_sf: "RP (sf_substate)"
+  using wf_world_model_def by auto
+
+lemma rp_enabled_iff:
+  assumes "RP M"
+  shows "plan_action_enabled \<pi> (M - sf_substate) \<longleftrightarrow> p2.plan_action_enabled \<pi> M"
+  using assms detyped_planaction_enabled_iff rp_props by auto
+
+(* TODO: lots of duplication from match_state_step*)
+lemma match_state_step':
+  assumes "states_match s s'" "p2.execute_plan_action \<pi> s' = t'" "p2.plan_action_enabled \<pi> s'"
+  shows "states_match (execute_plan_action \<pi> s) t'"
+proof -
+  obtain n args where pi: "\<pi> = PAction n args" by (cases \<pi>) simp
+  then obtain ac' where res': "p2.resolve_action_schema n = Some ac'"
+    using assms(3) p2.plan_action_enabled_def by fastforce
+  then obtain ac where res: "resolve_action_schema n = Some ac" and t_ac: "detype_classical_ac ac = ac'"
+    using t_resinst_inv by metis
+  hence 1: "effect (resolve_instantiate \<pi>) = map_ast_effect (ac_tsubst (ac_params ac) args) (ac_eff ac)"
+    using pi instantiate_action_schema_alt by simp
+  from res' have 2: "effect (p2.resolve_instantiate \<pi>) = map_ast_effect (ac_tsubst (ac_params ac') args) (ac_eff ac')"
+    using pi instantiate_action_schema_alt by simp
+
+  from t_ac have "map fst (ac_params ac) = map fst (ac_params ac')"
+    using t_ents_names detype_classical_ac_sel by metis
+  moreover from t_ac have "ac_eff ac = ac_eff ac'" by auto
+  ultimately have effeq: "effect (resolve_instantiate \<pi>) = effect (p2.resolve_instantiate \<pi>)"
+    using ac_tsubst_def 1 2 by force
+
+  from assms(1,3) have wf: "wf_plan_action \<pi>"
+    using detyped_planaction_enabled_iff plan_action_enabled_def by auto
+  hence "wf_ground_action (resolve_instantiate \<pi>)"
+    using wf_resolve_instantiate by simp
+  hence "wf_effect objT (effect (resolve_instantiate \<pi>))"
+    by (simp add: wf_ground_action_alt)
+  with sf_disj_wf_eff[OF this, where f = id] have
+    "sf_substate \<inter> set (adds (effect (resolve_instantiate \<pi>))) = {}"
+    "sf_substate \<inter> set (dels (effect (resolve_instantiate \<pi>))) = {}"
+    by (simp_all add: ast_effect.map_id)
+
+  hence "apply_effect (effect (resolve_instantiate \<pi>)) (s \<union> sf_substate) =
+    apply_effect (effect (resolve_instantiate \<pi>)) s \<union> sf_substate"
+    using 1 apply_effect_alt sf_disj_wf_wm by auto
+  hence "p2.execute_plan_action \<pi> s' = execute_plan_action \<pi> s \<union> sf_substate"
+    using effeq execute_plan_action_def
+    using p2.execute_plan_action_def assms(1) by simp
+  moreover have "wf_world_model (execute_plan_action \<pi> s)"
+    using wf_execute_stronger wf assms(1) by auto
+  ultimately show ?thesis using assms(2) by simp
+qed
+
+lemma match_valid_classical_plan_from2':
+  assumes "states_match s s'" "p2.valid_classical_plan_from2 s' \<pi>s"
+  shows "valid_classical_plan_from2 s \<pi>s"
+using assms proof (induction \<pi>s arbitrary: s s')
+  case Nil
+  hence "s' \<^sup>c\<TTurnstile>\<^sub>= goal P2"
+    using p2.valid_classical_plan_from2_def by simp
+  hence "s \<^sup>c\<TTurnstile>\<^sub>= goal P" using assms match_goal Nil.prems by simp
+  thus ?case using valid_classical_plan_from2_def by auto
+next
+  case (Cons p ps)
+  let ?t = "execute_plan_action p s"
+  let ?t' = "p2.execute_plan_action p s'"
+  from Cons have enab2: "p2.plan_action_enabled p s'" and valid2: "p2.valid_classical_plan_from2 ?t' ps"
+    using p2.valid_classical_plan_from2_def p2.plan_action_path_Cons by simp_all
+  from enab2 have enab1: "plan_action_enabled p s"
+    using detyped_planaction_enabled_iff assms(1) Cons.prems by simp
+  
+  have "states_match ?t ?t'"
+    using assms(1) enab2 match_state_step' Cons.prems by blast
+  hence "valid_classical_plan_from2 ?t ps"
+    using Cons.IH[OF _ valid2] by simp
+  with enab1 show ?case using valid_classical_plan_from2_def plan_action_path_Cons by simp
+qed
+
+lemma match_valid_classical_plan':
+  assumes "p2.valid_classical_plan2 \<pi>s"
+  shows "valid_classical_plan2 \<pi>s"
+  using assms unfolding valid_classical_plan2_def
+  using match_valid_classical_plan_from2' inits_match by blast
+
+(* putting it together: *)
+
+theorem detyped_valid_iff:
+  "valid_classical_plan2 \<pi>s \<longleftrightarrow> p2.valid_classical_plan2 \<pi>s"
+  using match_valid_classical_plan match_valid_classical_plan' by blast
+
+end
+
+subsection \<open> Code Setup \<close>
+
+lemmas type_norm_code =
+  ast_classical_domain.wf_action_params_def
+  ast_classical_domain.restrict_dom_def
+  ast_classical_domain.pred_for_type_def
+  ast_classical_domain.type_pred.simps
+  ast_classical_domain.type_preds_def
+  ast_classical_domain.type_atom.simps
+  ast_classical_domain.type_precond.simps
+  ast_classical_domain.param_precond_def
+  ast_classical_domain.detype_classical_ac.simps
+  ast_classical_domain.detype_classical_dom_def
+  ast_classical_domain.supertype_facts_for.simps
+  ast_classical_domain.supertype_facts_def
+  ast_classical_problem.detype_classical_prob_def
+  ast_classical_domain.typeless_dom_def
+  ast_classical_problem.typeless_prob_def
+declare type_norm_code[code]
+
+
+
+
+end
